lots of progress toward final theorem

Languages/Imp/Calc_Mem_Imp_Hoare_Example.thy
@@ -2,6 +2,7 @@ theory Calc_Mem_Imp_Hoare_Example
   imports Calc_Mem_Imp "../../Hoare/Hoare_Step" "../../Hoare/Hoare_Lift" 
     "../../Language_Components/Mem/Mem_Simple"
     "../../Lifter/Auto_Lifter_Proofs" "../../Composition/Composition_Lifter"
+    "Calc_Mem_Imp_Hoare"
 begin
 
 (* final definitions that perhaps should be in mem_simple (TODO) *)
@@ -58,56 +59,13 @@ lemma pres :
 "sups_pres sems (\<lambda> _ . ok_S)"
   by(rule sups_pres_finite_all; auto)
 
-(*
-proof(rule sups_presI)
-
-  fix x :: "('a, 'b) state"
-  fix sup :: "('a, 'b) state"
-  fix syn :: syn
-  fix Xs :: "('a, 'b) state set"
-  fix Fs' :: "(syn \<Rightarrow> ('a, 'b) state \<Rightarrow> ('a, 'b) state) set"
-  fix f :: "(syn \<Rightarrow> ('a, 'b) state \<Rightarrow> ('a, 'b) state)"
-  assume In_Xs : "x \<in> Xs"
-  assume Fin_Xs : "finite Xs"
-  assume Sup : "is_sup Xs sup"
-  assume Fs' : "Fs' \<subseteq> (sems :: (syn \<Rightarrow> ('a, 'b) state \<Rightarrow> ('a, 'b) state) set)"
-  assume "f \<in> Fs'"
-  show "\<exists>sup'.
-          is_sup ((\<lambda>f. f syn sup) ` Fs') sup' \<and> is_sup (scross ((\<lambda>f. f syn) ` Fs') Xs) sup'"
-    using Fs'
-    apply(auto simp add: is_sup_def is_least_def is_ub_def)
-  sorry
-*)
-
-(*
-lemma calc_dom :
-  "\<And> c . calc_sem_l \<downharpoonleft> sems_nos (Sc c)"
-  sorry
-
-lemma cond_dom :
-  "\<And> b . cond_sem_l \<downharpoonleft> sems_nos (Sb b)"
-  sorry
-
-lemma mem_dom :
-  "\<And> m . mem_sem_l \<downharpoonleft> sems_nos (Sm m)"
-  sorry
-
-lemma seq_dom :
-  "\<And> s . seq_sem_l \<downharpoonleft> sems (Ss s)"
-  sorry
-
-lemma imp_dom :
-  "\<And> i . imp_sem_l \<downharpoonleft> sems (Si i)"
-  sorry
-*)
-
 (* concrete state *)
 type_synonym cstate = "(syn, unit) Mem_Simple.state"
 
 definition start_state :: "syn gensyn \<Rightarrow> (syn, unit) Mem_Simple.state" where
 "start_state prog =
   ( Swr [prog]
-  , mdp 0 None
+  , mdp 0 (Some (mdt None))
   , Swr 0, Swr 0, Swr 0, Swr 0
   , Swr empty
   , ())"
@@ -172,275 +130,19 @@ definition prog1 :: "int \<Rightarrow> int \<Rightarrow> syn gensyn" where
   ]
 "
 
+(*
 term "sem_run sem_final"
 
 value "sem_run sem_final 100 (start_state prog0)"
 
-(* calc_sem_l and cond_sem_l
-*)
 value "sem_run (pcomps [calc_sem_l, mem_sem_l, seq_sem_l, cond_sem_l]) 100 (start_state prog_mini)"
 
 
 value "sem_run sem_final 100 (start_state prog_mini)"
 
 value "sem_run sem_final 100 (start_state (prog1 2 3))"
-
-(* quick n dirty approach: we should be able to get this information from the liftings,
-   but this requires more machinery *)
-(* TODO: change this to use liftings
-*)
-(*
-definition st_valid where
-"st_valid st = 
-  (case st of
-   (mdp _ (Some _), mdp _ (Some _)
-   ,mdp _ (Some _), _, _) \<Rightarrow> True
-   | _ \<Rightarrow> False)"
-  *)
-(*
-(* this will eventually be the valid-set for our lifting. *)
-consts state_S :: "syn \<Rightarrow> cstate set"
 *)
 
-(* ok great - so this finally works. now let's see if we can prove anything. *)
-
-declare [[show_types = false]]
-declare [[show_sorts = false]]
-
-(* individual pieces.
-*)
-
-lemma HCalc_calc :
-  assumes Hc : "c \<noteq> Cskip"
-  shows "Calc.calc_sem % {{P1}} c
-                         {{(\<lambda> st . case st of
-                              (x1, x2, x3) \<Rightarrow> 
-                              (\<exists> x3' . P1 (x1, x2, x3')) \<and>
-                              (\<forall> x3' . calc_sem c (x1, x2, x3') = st))}}"
-proof(rule HTSI)
-  fix a
-  assume H : "P1 a"
-
-  show "case calc_sem c a of (x1, x2, x3) \<Rightarrow> (\<exists>x3'. P1 (x1, x2, x3')) \<and> (\<forall>x3'. calc_sem c (x1, x2, x3') = calc_sem c a)"
-    using Hc H
-    by(cases c; cases a; auto simp add: split: prod.splits)
-qed
-
-lemma HCond_cond :
-  assumes Hc : "c \<noteq> Cond.Sskip_cond"
-  shows "Cond.cond_sem % {{P1}} c
-                         {{(\<lambda> st . case st of
-                              (x1, x2) \<Rightarrow> 
-                              (\<exists> x1' . P1 (x1', x2)) \<and>
-                              (\<forall> x1' . cond_sem c (x1', x2) = st))}}"
-proof(rule HTSI)
-  fix a
-  assume H : "P1 a"
-
-  show "case cond_sem c a of
-         (x1, x2) \<Rightarrow> (\<exists>x1'. P1 (x1', x2)) \<and> (\<forall>x1'. cond_sem c (x1', x2) = cond_sem c a)"
-    using Hc H
-    by(cases c; cases a; auto simp add: cond_sem_def split: prod.splits)
-qed
-
-
-(* need to push through lifting first. *)
-(*
-lemma HCalc_calc' :
-  fixes P1
-  assumes Hc : "c \<noteq> Cskip"
-  shows "Calc.calc_sem % {{P1}} c
-                         {{(\<lambda> X st . case st of
-                              (x1, x2, x3) \<Rightarrow> 
-                              (\<exists> x3' . X (x1, x2, x3')) \<and>
-                              (\<forall> x3' . calc_sem c (x1, x2, x3') = st)) P1}}"
-  using HCalc_calc Hc
-  by auto
-*)
-(*declare [[show_sorts]]*)
-(* problem here is with where the syntax translation is happening, I think. *)
-
-(*
-term "calc_lift"
-lemma HCalc_calc'' :
-  fixes P' :: "('a, ('b :: {Okay,Bogus,Mergeableb})) state \<Rightarrow> bool"
-  assumes Hv : "  lifting_valid (calc_lift :: (calc, calc_state, ('a, 'b) state) lifting) S"
-  assumes Hs : "Calc_Mem_Imp.calc_trans x' = c"
-  assumes Hc : "c \<noteq> Cskip"
-  shows "Calc_Mem_Imp.calc_sem_l % {{P'}} x' {{liftt_conc
-         Calc_Mem_Imp.calc_trans calc_lift x'
-         (\<lambda>P st.
-             case st of
-             (x1, x2, x3) \<Rightarrow>
-               (\<exists>x3'. P (x1, x2, x3')) \<and>
-               (\<forall>x3'. calc_sem c (x1, x2, x3') = st))
-         P'}}"
-  using assms liftt_conc_spec[OF _ HCalc_calc'[OF Hc], of calc_lift _ calc_trans _,
-      folded calc_sem_l_def, OF Hv Hs, of P']
-  by auto
-*)
-(* next: if P' implies OK, then liftt_conc of P'
-will also be OK (assuming valid lifting)
-*)
-
-(*
-lemma whoa :
-    assumes "liftt_conc
-         Calc_Mem_Imp.calc_trans calc_lift x'
-         (\<lambda>P st.
-             case st of
-             (x1, x2, x3) \<Rightarrow>
-               (\<exists>x3'. P (x1, x2, x3')) \<and>
-               (\<forall>x3'. calc_sem c (x1, x2, x3') = st))
-         P' st = z"
-    shows False using assms
-  apply(auto simp add: liftt_conc_def calc_lift_def)
-  *)
-
-  
-(*
-  have False
-    using liftt_conc_spec[OF _ HCalc_calc'[OF Hc], of calc_lift _ calc_trans _,
-folded calc_sem_l_def]
-*)
-  
-
-
-lemma HCalc_skip :
-  shows "Calc.calc_sem % {{P1}} Cskip
-                         {{P1}}"
-proof(rule HTSI)
-  fix a
-  assume H : "P1 a"
-
-  show "P1 (calc_sem Cskip a)"
-    using H
-    by(cases a; auto simp add: split: prod.splits)
-qed
-
-lemma HCalc_Cnum :
-  shows "Calc.calc_sem % {{P1}} (Cnum i)
-         {{(\<lambda> st . 
-            case st of (c1, c2, x) \<Rightarrow> x = i \<and> (\<exists> old . P1 (c1, c2, old)))}}"
-proof(rule HTSI)
-  fix a
-  assume H : "P1 a"
-
-  show "case calc_sem (Cnum i) a of
-         (c1, c2, x) \<Rightarrow>
-           x = i \<and>
-           (\<exists>old. P1 (c1, c2, old))" using H
-    by(cases a; auto simp add: split: prod.splits)
-qed
-
-lemma HCalc_Cadd :
-  shows "Calc.calc_sem % {{P1}} (Cadd)
-         {{(\<lambda> st . 
-            case st of (c1, c2, x) \<Rightarrow> x = c1 + c2 \<and> 
-            (\<exists> old . P1 (c1, c2, old)))}}"
-proof(rule HTSI)
-  fix a
-  assume H : "P1 a"
-
-  show "case calc_sem Cadd a of
-         (c1, c2, x) \<Rightarrow>
-           x = c1 + c2 \<and>
-           (\<exists>old. P1 (c1, c2, old))" using H
-    by(cases a; auto simp add: split: prod.splits)
-qed
-
-(* HCalc_Csub *)
-lemma HCalc_Csub :
-  shows "Calc.calc_sem % {{P1}} (Csub)
-         {{(\<lambda> st . 
-            case st of (c1, c2, x) \<Rightarrow> x = c1 - c2 \<and> 
-            (\<exists> old . P1 (c1, c2, old)))}}"
-proof(rule HTSI)
-  fix a
-  assume H : "P1 a"
-
-  show "case calc_sem Csub a of
-         (c1, c2, x) \<Rightarrow>
-           x = c1 - c2 \<and>
-           (\<exists>old. P1 (c1, c2, old))" using H
-    by(cases a; auto simp add: split: prod.splits)
-qed
-
-lemma HCalc_Cmul :
-  shows "Calc.calc_sem % {{P1}} (Cmul)
-         {{(\<lambda> st . 
-            case st of (c1, c2, x) \<Rightarrow> x = c1 * c2 \<and> 
-            (\<exists> old . P1 (c1, c2, old)))}}"
-proof(rule HTSI)
-  fix a
-  assume H : "P1 a"
-
-  show "case calc_sem Cmul a of
-         (c1, c2, x) \<Rightarrow>
-           x = c1 * c2 \<and>
-           (\<exists>old. P1 (c1, c2, old))" using H
-    by(cases a; auto simp add: split: prod.splits)
-qed
-
-lemma HCond_Seqz :
-  shows "Cond.cond_sem % {{P1}} (Seqz)
-          {{(\<lambda> st . 
-              case st of (c, i) \<Rightarrow> c = encode_bool (i = 0) \<and>
-                (\<exists> old . P1 (old, i)))}}"
-proof(rule HTSI)
-  fix a
-  assume H : "P1 a"
-
-  show "case cond_sem Seqz a of
-         (c, i) \<Rightarrow>
-           c = encode_bool (i = 0) \<and>
-           (\<exists>old. P1 (old, i))" using H
-    by(cases a; auto simp add: cond_sem_def)
-qed
-
-lemma HCond_Sltz :
-  shows "Cond.cond_sem % {{P1}} (Sltz)
-          {{(\<lambda> st . 
-              case st of (c, i) \<Rightarrow> c = encode_bool (i < 0) \<and>
-                (\<exists> old . P1 (old, i)))}}"
-proof(rule HTSI)
-  fix a
-  assume H : "P1 a"
-
-  show "case cond_sem Sltz a of
-         (c, i) \<Rightarrow>
-           c = encode_bool (i < 0) \<and>
-           (\<exists>old. P1 (old, i))" using H
-    by(cases a; auto simp add: cond_sem_def)
-qed
-
-lemma HCond_Sgtz :
-  shows "Cond.cond_sem % {{P1}} (Sgtz)
-          {{(\<lambda> st . 
-              case st of (c, i) \<Rightarrow> c = encode_bool (i > 0) \<and>
-                (\<exists> old . P1 (old, i)))}}"
-proof(rule HTSI)
-  fix a
-  assume H : "P1 a"
-
-  show "case cond_sem Sgtz a of
-         (c, i) \<Rightarrow>
-           c = encode_bool (i > 0) \<and>
-           (\<exists>old. P1 (old, i))" using H
-    by(cases a; auto simp add: cond_sem_def)
-qed
-
-lemma HCond_skip :
-  shows "Cond.cond_sem % {{P1}} Sskip_cond
-                         {{P1}}"
-proof(rule HTSI)
-  fix a
-  assume H : "P1 a"
-
-  show "P1 (cond_sem Sskip_cond a)"
-    using H
-    by(cases a; auto simp add: cond_sem_def split: prod.splits)
-qed
 
 definition oalist_check' :: "('a :: linorder * 'b md_triv option md_prio) list \<Rightarrow> bool"
   where
@@ -492,484 +194,10 @@ proof-
     by(auto simp add: pred_option_def)
 qed
 
-(*
-definition mem_ok :: "('s, 'x) Mem_Simple.state \<Rightarrow> bool" where
-"mem_ok st =
-  (case st of
-    ((mdp _ (Some (mdt _)))
-    , (mdp _ None)
-    , (mdp _ (Some (mdt _)))
-    , (mdp _ (Some (mdt _)))
-    , (mdp _ (Some (mdt _)))
-    , (mdp _ (Some (mdt _)))
-    , (mdp _ (Some (mdt l)))
-    , _) \<Rightarrow> oalist_check l
-    | _ \<Rightarrow> False)"
-
-
-definition mem_unwrap :: "('s, 'x) Mem_Simple.state \<Rightarrow> Mem_Simple.state0 option"
-where
-"mem_unwrap st =
- (case st of
-    ((mdp _ (Some (mdt _)))
-    , (mdp _ None)
-    , (mdp _ (Some (mdt reg_flag)))
-    , (mdp _ (Some (mdt reg_c)))
-    , (mdp _ (Some (mdt reg_a)))
-    , (mdp _ (Some (mdt reg_b)))
-    , l
-    , _) \<Rightarrow> 
-      (case oalist_unwrap l of
-       Some l' \<Rightarrow> Some (reg_flag, reg_c, reg_a, reg_b, l')
-       | None \<Rightarrow> None)
-    | _ \<Rightarrow> None)"
-*)  
-(* Mem_Read *)
-(*
-need to figure out a couple of things
-1. should we have the predicate P1 be over the inner data, or the "raw" wrapped data? 
-2. how to handle the different cases about whether there was or wasn't a value at that location before?
-   (this is more of a concern for write)
-*)
-
-lemma HMem_Sread :
-  shows "mem0_sem % {{ P1 }} (Sread s r)
-                   {{ (\<lambda> st .
-                        (case st of (reg_flag, reg_c, reg_a, reg_b, m) \<Rightarrow>
-                          (case get m s of
-                           Some v \<Rightarrow> 
-                           (case r of Reg_a \<Rightarrow> reg_a = v \<and> (\<exists> old . P1 (reg_flag, reg_c, old, reg_b, m))
-                                      | Reg_b \<Rightarrow> reg_b = v \<and> (\<exists> old . P1 (reg_flag, reg_c, reg_a, old, m))
-                                      | Reg_c \<Rightarrow> reg_c = v \<and> (\<exists> old . P1 (reg_flag, old, reg_a, reg_b, m))
-                                      | Reg_flag \<Rightarrow> reg_flag = v \<and> (\<exists> old . P1 (old, reg_c, reg_a, reg_b, m)))
-                            | None \<Rightarrow> P1 st))) }}"
-proof(rule HTSI)      
-  fix a
-  assume H : "P1 a"
-
-  obtain reg_flag reg_c reg_a reg_b m where
-    A : "a = (reg_flag, reg_c, reg_a, reg_b, m)"
-    by(cases a; auto)
-
-  obtain reg_flag' reg_c' reg_a' reg_b' m' where
-    Result : "mem0_sem (Sread s r) a = (reg_flag', reg_c', reg_a', reg_b', m')"
-    by(cases "mem0_sem (Sread s r) a"; auto)
-
-  show "case mem0_sem (Sread s r) a of
-         (reg_flag, reg_c, reg_a, reg_b, m) \<Rightarrow>
-           (case get m s of None \<Rightarrow> P1 (mem0_sem (Sread s r) a)
-             | Some v \<Rightarrow>
-                 (case r of
-                   Reg_a \<Rightarrow>
-                     reg_a = v \<and>
-                     (\<exists>old. P1 (reg_flag, reg_c, old, reg_b, m))
-                   | Reg_b \<Rightarrow>
-                       reg_b = v \<and>
-                       (\<exists>old. P1 (reg_flag, reg_c, reg_a, old, m))
-                   | Reg_c \<Rightarrow>
-                       reg_c = v \<and>
-                       (\<exists>old. P1 (reg_flag, old, reg_a, reg_b, m))
-                   | Reg_flag \<Rightarrow>
-                       reg_flag = v \<and>
-                       (\<exists>old. P1 (old, reg_c, reg_a, reg_b, m))))"
-  proof(cases "get m s")
-    case None
-
-    then show ?thesis
-      using H Result A
-      by(auto split: option.splits reg_id.splits)
-  next
-    case (Some v)
-    then show ?thesis using H Result A
-      by(auto split: option.splits reg_id.splits)
-  qed
-qed
-
-
-lemma str_ord_undo_update1 :
-  assumes H : "strict_order (map fst l)"
-  assumes Hget : "map_of l k = None"
-  shows "str_ord_delete k (str_ord_update k v l) = l"
-  using assms
-proof(induction l)
-  case Nil
-  then show ?case
-    by auto
-next
-  case (Cons h l)
-
-  obtain hk hv where Hkv : "h = (hk, hv)"
-    by(cases h; auto)
-
-  have Ord' : "strict_order (map fst l)"
-    using Cons.prems(1) strict_order_tl[of hk "map fst l"]
-    unfolding Hkv
-    by auto
-
-  show ?case
-  proof(cases "k = hk")
-    case True
-    then show ?thesis using Cons Hkv by auto
-  next
-    case False
-    then show ?thesis using Cons.prems Cons.IH[OF Ord'] Hkv
-      by(auto)
-  qed
-qed
-
-lemma undo_update1 :
-  "get m k = None \<Longrightarrow> delete k (update k v m) = m"
-  by(transfer; auto intro: str_ord_undo_update1)              
-
-lemma str_ord_undo_update2 :
-  assumes H : "strict_order (map fst l)"
-  assumes Hget : "map_of l k = Some v"
-  shows "str_ord_update k v (str_ord_update k v' l) = l"
-  using assms
-proof(induction l)
-  case Nil
-  then show ?case
-    by auto
-next
-  case (Cons h l)
-
-  obtain hk hv where Hkv : "h = (hk, hv)"
-    by(cases h; auto)
-
-  have Ord' : "strict_order (map fst l)"
-    using Cons.prems(1) strict_order_tl[of hk "map fst l"]
-    unfolding Hkv
-    by auto
-
-  show ?case
-  proof(cases "k = hk")
-    case True
-    then show ?thesis using Cons Hkv by auto
-  next
-    case False
-
-    have Hget' : "map_of l k = Some v"
-      using Cons.prems Cons.IH[OF Ord'] Hkv False
-      by(auto)
-
-    have Hget'' : "(k, v) \<in> set l"
-      using map_of_SomeD[OF Hget'] by simp
-
-    then obtain idx where Get_idx : "l ! idx = (k, v)" "idx < length l"
-      unfolding in_set_conv_nth by auto
-
-    show ?thesis 
-      using Hkv False Cons.prems strict_order_unfold[OF Cons.prems(1), of "idx + 1" 0] Get_idx
-        Cons.IH[OF Ord']
-      by(auto)
-  qed
-qed
-
-lemma undo_update2 :
-  "get m k = Some v \<Longrightarrow> update k v (update k v' m) = m"
-  by(transfer; auto intro: str_ord_undo_update2)              
-
-lemma str_ord_update_noop :
-  assumes H : "strict_order (map fst l)"
-  assumes Hget : "map_of l k = Some v"
-  shows "str_ord_update k v l = l" using assms
-proof(induction l)
-  case Nil
-  then show ?case 
-    by auto
-next
-  case (Cons h l)
-
-  obtain hk hv where Hkv : "h = (hk, hv)"
-    by(cases h; auto)
-
-  have Ord' : "strict_order (map fst l)"
-    using Cons.prems(1) strict_order_tl[of hk "map fst l"]
-    unfolding Hkv
-    by auto
-
-  show ?case
-  proof(cases "k = hk")
-    case True
-    then show ?thesis using Cons Hkv by auto
-  next
-    case False
-    have Hget' : "map_of l k = Some v"
-      using Cons.prems Cons.IH[OF Ord'] Hkv False
-      by(auto)
-
-    have Hget'' : "(k, v) \<in> set l"
-      using map_of_SomeD[OF Hget'] by simp
-
-    then obtain idx where Get_idx : "l ! idx = (k, v)" "idx < length l"
-      unfolding in_set_conv_nth by auto
-
-    show ?thesis 
-      using Hkv False Cons.prems strict_order_unfold[OF Cons.prems(1), of "idx + 1" 0] Get_idx
-        Cons.IH[OF Ord']
-      by(auto)
-  qed
-qed
-
-lemma update_noop :
-  assumes Hget : "get l k = Some v"
-  shows "update k v l = l" using assms
-  by(transfer; auto intro: str_ord_update_noop)              
-
-lemma HMem_Swrite :
-  shows "mem0_sem % {{ P1 }} (Swrite s r)
-                    {{ (\<lambda> st . 
-                        (case st of (reg_flag, reg_c, reg_a, reg_b, m) \<Rightarrow>
-                          (case r of
-                            Reg_a \<Rightarrow> get m s = Some reg_a
-                            | Reg_b \<Rightarrow> get m s = Some reg_b
-                            | Reg_c \<Rightarrow> get m s = Some reg_c
-                            | Reg_flag \<Rightarrow> get m s = Some reg_flag) \<and>
-                          (((\<exists>old. P1 (reg_flag, reg_c, reg_a, reg_b, update s old m)) \<or>
-                           (P1 (reg_flag, reg_c, reg_a, reg_b, delete s m)))))) }}"
-proof(rule HTSI)
-  fix a
-
-  assume H: "P1 a"
-
-  show "case mem0_sem (Swrite s r) a of
-         (reg_flag, reg_c, reg_a, reg_b, m) \<Rightarrow>
-           (case r of
-             Reg_a \<Rightarrow>
-               get m s = Some reg_a 
-             | Reg_b \<Rightarrow>
-                 get m s = Some reg_b
-             | Reg_c \<Rightarrow>
-                 get m s = Some reg_c
-             | Reg_flag \<Rightarrow>
-                 get m s = Some reg_flag) \<and>
-             ((\<exists>old. P1 (reg_flag, reg_c, reg_a, reg_b, update s old m)) \<or>
-             (P1 (reg_flag, reg_c, reg_a, reg_b, delete s m))) "
-  proof-
-  
-    obtain reg_flag reg_c reg_a reg_b m where
-      A : "a = (reg_flag, reg_c, reg_a, reg_b, m)"
-      by(cases a; auto)
-  
-    obtain reg_flag' reg_c' reg_a' reg_b' m' where
-      Result : "mem0_sem (Swrite s r) a = (reg_flag', reg_c', reg_a', reg_b', m')"
-      by(cases "mem0_sem (Swrite s r) a"; auto)
-  
-    show ?thesis
-    proof(cases "get m s")
-      case None
-      then show ?thesis using A Result H undo_update1[OF None]
-        by(cases r; auto simp add: get_update update_update)
-    next
-      case (Some v)
-  
-      have Conc' :
-        "P1 (reg_flag', reg_c', reg_a', reg_b', update s v m)"
-        using A Result H update_noop[OF Some]
-        by(cases r; auto simp add: get_update update_update )
-  
-      then show ?thesis using A Result H update_noop[OF Some]
-        by(cases r; auto simp add: get_update update_update; blast)
-    qed 
-  qed
-qed
-
-(*
-
-*)
-
-term "sem_final"
-
-definition calc_lift' where
-"calc_lift' =  (schem_lift (SP NA (SP NB NC)) (SP NX (SP (SPRC calc_prio (SO NC)) (SP (SPRI (SO NA)) (SP (SPRI (SO NB)) NX)))))"
-
-term "mem_sem_lifting_gen"
-term "calc_lift'"
-(* TODO: the requirement that new and old reg_a and reg_b be equal is a hack. *)
-lemma Calc_Final : 
-  fixes gs :: "syn \<Rightarrow> (syn, (_ ::{Okay,Mergeableb,Bogus})) state \<Rightarrow> (syn, (_ ::{Okay,Bogus,Mergeableb})) state"
-  assumes P1_ok : "\<And> st . P st \<Longrightarrow> st \<in> ok_S"
-  assumes HP : "\<And> st . P st \<Longrightarrow> P' (LOut calc_lift' y st)"
-
-  shows "|gs| {~ (\<lambda> st . P st) ~} [G (Sc y) z] 
-    {~ (\<lambda> st . \<exists> old_big small_new . P old_big \<and> (case small_new of
-                                  (x1, x2, x3) \<Rightarrow>
-                                    (\<exists>x3'. P' (x1, x2, x3')) \<and>
-                                    (\<forall>x3'. calc_sem y (x1, x2, x3') = small_new)) \<and>
-                                 st = LUpd calc_lift' y small_new old_big) ~}"
-  apply(rule HTS_imp_HT'')
-            apply(rule_tac HCalc_calc)
-  sorry
-
-(* Allows us to use the fact that the original inputs are unchanged.
- * if this ends up helping we need to find a way to generalize/standardize this. *)
-lemma Add_Final : 
-  fixes gs :: "syn \<Rightarrow> (syn, (_ ::{Okay,Mergeableb,Bogus})) state \<Rightarrow> (syn, (_ ::{Okay,Bogus,Mergeableb})) state"
-  assumes P1_ok : "\<And> st . P st \<Longrightarrow> st \<in> ok_S"
-  assumes HP : "\<And> st . P st \<Longrightarrow> P' (LOut calc_lift' Cadd st)"
-
-  shows "|gs| {~ (\<lambda> st . P st) ~} [G (Sc (Cadd)) z] 
-    {~ (\<lambda> st . \<exists> old_big small_new . P old_big \<and> (case small_new of
-                                  (c1, c2, x) \<Rightarrow> x = c1 + c2 \<and> (\<exists>old. P' (c1, c2, old) \<and> LOut calc_lift' Cadd old_big = (c1, c2, old))) \<and>
-                                 st = LUpd calc_lift' Cadd small_new old_big) ~}"
-(*  apply(rule HTS_imp_HT'') *)
-(*            apply(rule_tac HCalc_Cadd) *)
-  sorry
-
-lemma Sub_Final : 
-  fixes gs :: "syn \<Rightarrow> (syn, (_ ::{Okay,Mergeableb,Bogus})) state \<Rightarrow> (syn, (_ ::{Okay,Bogus,Mergeableb})) state"
-  assumes P1_ok : "\<And> st . P st \<Longrightarrow> st \<in> ok_S"
-  assumes HP : "\<And> st . P st \<Longrightarrow> P' (LOut calc_lift' Csub st)"
-
-  shows "|gs| {~ (\<lambda> st . P st) ~} [G (Sc (Csub)) z] 
-    {~ (\<lambda> st . \<exists> old_big small_new . P old_big \<and> (case small_new of
-                                  (c1, c2, x) \<Rightarrow> x = c1 - c2 \<and> (\<exists>old. P' (c1, c2, old) \<and> LOut calc_lift' Cadd old_big = (c1, c2, old))) \<and>
-                                 st = LUpd calc_lift' Csub small_new old_big) ~}"
-(*  apply(rule HTS_imp_HT'') *)
-(*            apply(rule_tac HCalc_Cadd) *)
-  sorry
-
-
-definition cond_lift' where
-"cond_lift' = (schem_lift (SP NA NB) (SP (SPRC cond_prio (SO NA)) (SP (SPRK (SO NB)) NX)))"
-
-lemma Cond_Final : 
-  fixes gs :: "syn \<Rightarrow> (syn, (_ ::{Okay,Mergeableb,Bogus})) state \<Rightarrow> (syn, (_ ::{Okay,Bogus,Mergeableb})) state"
-  assumes P1_ok : "\<And> st . P st \<Longrightarrow> st \<in> ok_S"
-  assumes HP : "\<And> st . P st \<Longrightarrow> P' (LOut cond_lift' y st)"
-
-  shows "|gs| {~ (\<lambda> st . P st) ~} [G (Sb y) z] 
-    {~ (\<lambda> st . \<exists> old_big small_new . P old_big \<and> (case small_new of
-                                  (x1', x2) \<Rightarrow>
-                                    (\<exists>x1'. P' (x1', x2) ) \<and>
-                                    (\<forall>x1'. cond_sem y (x1', x2) = small_new)) \<and>
-                                 st = LUpd cond_lift' y small_new old_big) ~}"
-  apply(rule HTS_imp_HT'')
-            apply(rule_tac HCond_cond)
-  sorry
-
-(* As with arith. Need to see if we can standardize this. *)
-lemma Gtz_Final :
-  fixes gs :: "syn \<Rightarrow> (syn, (_ ::{Okay,Mergeableb,Bogus})) state \<Rightarrow> (syn, (_ ::{Okay,Bogus,Mergeableb})) state"
-  assumes P1_ok : "\<And> st . P st \<Longrightarrow> st \<in> ok_S"
-  assumes HP : "\<And> st . P st \<Longrightarrow> P' (LOut cond_lift' (Sgtz) st)"
-
-  shows "|gs| {~ (\<lambda> st . P st) ~} [G (Sb y) z] 
-    {~ (\<lambda> st . \<exists> old_big small_new . P old_big \<and> (case small_new of
-                                  (x1', x2) \<Rightarrow> x1' = encode_bool (x2 > 0) \<and> (\<exists> old . P' (old, x2) \<and> LOut cond_lift' Sgtz (old_big) = (old, x2)))
-                                    \<and>
-                                 st = LUpd cond_lift' Sgtz small_new old_big) ~}"
-  sorry
-
-
-(* TODO: correctly capture case where variable is empty 
- * do we need HGet, or don't we?*)
-lemma Mem_Read_Final : 
-  fixes gs :: "syn \<Rightarrow> (syn, (_ ::{Okay,Mergeableb,Bogus})) state \<Rightarrow> (syn, (_ ::{Okay,Bogus,Mergeableb})) state"
-  assumes P1_ok : "\<And> st . P st \<Longrightarrow> st \<in> ok_S"
-  assumes HP : "\<And> st . P st \<Longrightarrow> P' (LOut mem_lift1 (Sread v r) st)"
-(*
-  assumes Hget : "\<And> st . P st \<Longrightarrow>
-    (case st of (_, _, _, _, m, _) \<Rightarrow>
-      (case m of
-        mdp p (Some (mdt m')) \<Rightarrow> 
-          (case get m' v of
-            Some _ \<Rightarrow> True
-            | _ \<Rightarrow> False)
-         | _ \<Rightarrow> False))"
-*)
-(*
-  shows "|gs| {~ (\<lambda> st . P st) ~} [G (Sm (Sread v r)) z] 
-    {~ (\<lambda> st . \<exists> old_big small_new . P old_big \<and> (case small_new of
-                                  (reg_flag, reg_c, reg_a, reg_b, m) \<Rightarrow>
-                                        case get m ?s of None \<Rightarrow> ?P1.0 st
-                                        | Some v \<Rightarrow>
-                                            case ?r of Reg_a \<Rightarrow> reg_a = v \<and> (\<exists>old. ?P1.0 (reg_flag, reg_c, old, reg_b, m))
-                                            | Reg_b \<Rightarrow> reg_b = v \<and> (\<exists>old. ?P1.0 (reg_flag, reg_c, reg_a, old, m)) | Reg_c \<Rightarrow> reg_c = v \<and> (\<exists>old. ?P1.0 (reg_flag, old, reg_a, reg_b, m))
-                                            | Reg_flag \<Rightarrow> reg_flag = v \<and> (\<exists>old. ?P1.0 (old, reg_c, reg_a, reg_b, m))) \<and>
-                                 st = LUpd mem_sem_lifting_inner y small_new old_big) ~}"
-*)
-shows " |gs| {~P~} [G (Calc_Mem_Imp.syn.Sm (Sread v r))
-                 z] {~(\<lambda>st. \<exists>old_big small_new.
-                                 P old_big \<and>
-                                 (case small_new of
-(reg_flag, reg_c, reg_a, reg_b, m) \<Rightarrow>
-  case get m v of None \<Rightarrow> False
-  | Some v \<Rightarrow>
-      case r of Reg_a \<Rightarrow> reg_a = v \<and> (\<exists>old. P' (reg_flag, reg_c, old, reg_b, m))
-      | Reg_b \<Rightarrow> reg_b = v \<and> (\<exists>old. P' (reg_flag, reg_c, reg_a, old, m))
-      | Reg_c \<Rightarrow> reg_c = v \<and> (\<exists>old. P' (reg_flag, old, reg_a, reg_b, m))
-      | Reg_flag \<Rightarrow> reg_flag = v \<and> (\<exists>old. P' (old, reg_c, reg_a, reg_b, m))) \<and>
-                                 st =
-                                 LUpd mem_lift1 (Sread v r) small_new
-old_big)~}"
-  using HTS_imp_HT''[where l' = mem_trans, where x = "Sm (Sread v r)",
-unfolded mem_trans.simps, OF HMem_Sread]
-
-  sorry
-
-(* TODO: write version of Read_Final lemma *)
-lemma Mem_Write_Final : 
-  fixes gs :: "syn \<Rightarrow> (syn, (_ ::{Okay,Mergeableb,Bogus})) state \<Rightarrow> (syn, (_ ::{Okay,Bogus,Mergeableb})) state"
-  assumes P1_ok : "\<And> st . P st \<Longrightarrow> st \<in> ok_S"
-  assumes HP : "\<And> st . P st \<Longrightarrow> P' (LOut mem_lift1 (Swrite v r) st)"
-
-(*
-  shows "|gs| {~ (\<lambda> st . P st) ~} [G (Sm (Sread v r)) z] 
-    {~ (\<lambda> st . \<exists> old_big small_new . P old_big \<and> (case small_new of
-                                  (reg_flag, reg_c, reg_a, reg_b, m) \<Rightarrow>
-                                        case get m ?s of None \<Rightarrow> ?P1.0 st
-                                        | Some v \<Rightarrow>
-                                            case ?r of Reg_a \<Rightarrow> reg_a = v \<and> (\<exists>old. ?P1.0 (reg_flag, reg_c, old, reg_b, m))
-                                            | Reg_b \<Rightarrow> reg_b = v \<and> (\<exists>old. ?P1.0 (reg_flag, reg_c, reg_a, old, m)) | Reg_c \<Rightarrow> reg_c = v \<and> (\<exists>old. ?P1.0 (reg_flag, old, reg_a, reg_b, m))
-                                            | Reg_flag \<Rightarrow> reg_flag = v \<and> (\<exists>old. ?P1.0 (old, reg_c, reg_a, reg_b, m))) \<and>
-                                 st = LUpd mem_sem_lifting_inner y small_new old_big) ~}"
-*)
-shows " |gs| {~P~} [G (Calc_Mem_Imp.syn.Sm (Swrite v r))
-                 z] {~(\<lambda>st. \<exists>old_big small_new.
-                                 P old_big \<and>
-                                 (case small_new of
-                                  (reg_flag, reg_c, reg_a, reg_b, m) \<Rightarrow>
-                                    (case r of Reg_a \<Rightarrow> get m v = Some reg_a
-                                     | Reg_b \<Rightarrow> get m v = Some reg_b
-                                     | Reg_c \<Rightarrow> get m v = Some reg_c
-                                     | Reg_flag \<Rightarrow> get m v = Some reg_flag) \<and>
-                                    ((\<exists>old. P' (reg_flag, reg_c, reg_a, reg_b,
- update v old m)) \<or>
-                                     P' (reg_flag, reg_c, reg_a, reg_b, delete v m))) \<and>
-                                 st = LUpd mem_lift1 (Swrite v r) small_new old_big)~}"
-  using HTS_imp_HT''[where l' = mem_trans, where x = "Sm (Swrite v r)",
-unfolded mem_trans.simps, OF HMem_Swrite]
-
-  sorry
-
-(* TODO: need to figure out how the lifting works. *)
-
-(*
-lemma Merge_Out :
-  shows "LOut (merge_l l1 l2) = (\<lambda> a b . (LOut (fst_l l1) a b, LOut (snd_l l2) a b))"
-
-  term "l2"
-  sorry
-*)
-
-(* now need a sequencing stepping lemma. *)
 
 lemma prog1_spec :
   assumes Hi1 : "0 < i1" (* TODO: this should be \<le>, but for (i think) a technical reason this makes things hard (existential quantifier related problems) *)
   assumes Hi2 : "0 \<le> i2"
-
-(* TODO: st_valid need to be replaced *)
-
-(* ok, st_valid should be somethng like (is in a valid_s of some kind) *)
-
-(* use Ok here.
-problem: will this be enough? or will we still need to figure out how to "frame out" everything else?
-*)
-
-(* need to make these a bit more ergonomic, but hopefully they will work.
-one approach would be to special case this for each rule.
- *)
 
 (* prog1 *)
 (*
@@ -1011,25 +239,16 @@ proof-
 
     apply(rule HT'Conseq)
       apply(rule_tac P' = "\<lambda> _ . True" in Calc_Final)
-       apply(fast) apply(fast) apply(fast)
+       apply(fast) apply(fast)
+    apply(force  simp add: calc_lift'_def schem_lift_defs merge_l_def
+fst_l_def snd_l_def prio_l_def option_l_def triv_l_def 
+option_ok_S prod_ok_S prio_ok_S triv_ok_S)
+     apply(fast)
     apply(force  simp add: calc_lift'_def schem_lift_defs merge_l_def
 fst_l_def snd_l_def prio_l_def option_l_def triv_l_def 
 option_ok_S prod_ok_S prio_ok_S triv_ok_S)
     done
 
-(*
-(\<lambda>st. \<exists>old_big small_new.
-                                 P old_big \<and>
-                                 (case small_new of
-                                  (reg_flag, reg_c, reg_a, reg_b, m) \<Rightarrow>
-                                    (case r of Reg_a \<Rightarrow> get m v = Some reg_a | Reg_b \<Rightarrow> get m v = Some reg_b
-                                     | Reg_c \<Rightarrow> get m v = Some reg_c | Reg_flag \<Rightarrow> get m v = Some reg_flag) \<and>
-                                    ((\<exists>old. True) \<or> True)) \<and>
-                                 st = LUpd mem_lift1 (Swrite v r) small_new old_big
-*)
-
-(* NB: this used to work before we plugged in i1, but that is what we really want here. *)
-(* TODO: need oalist zip vs get lemma *)
   have 2 : "|sem_final| 
     {~ ?P1 ~}
     [G (Sm (Swrite (STR ''arg1'') (Reg_c))) []]
@@ -1093,7 +312,12 @@ fst_l_def snd_l_def prio_l_def option_l_def triv_l_def
 option_ok_S prod_ok_S prio_ok_S triv_ok_S oalist_ok_S
  LNew_def
 split: md_triv.splits) 
-
+  apply(force simp add: calc_lift'_def schem_lift_defs merge_l_def mem_lift1_def
+mem_sem_lifting_inner_def
+fst_l_def snd_l_def prio_l_def option_l_def triv_l_def 
+option_ok_S prod_ok_S prio_ok_S triv_ok_S oalist_ok_S
+ LNew_def
+split: md_triv.splits) 
     done
 
   have 4 : "|sem_final| 
@@ -1169,6 +393,12 @@ option_ok_S prod_ok_S prio_ok_S triv_ok_S oalist_ok_S
  LNew_def
 split: md_triv.splits) 
 
+  apply(force simp add: calc_lift'_def schem_lift_defs merge_l_def mem_lift1_def
+mem_sem_lifting_inner_def
+fst_l_def snd_l_def prio_l_def option_l_def triv_l_def
+option_ok_S prod_ok_S prio_ok_S triv_ok_S oalist_ok_S
+ LNew_def
+split: md_triv.splits) 
   apply(force simp add: calc_lift'_def schem_lift_defs merge_l_def mem_lift1_def
 mem_sem_lifting_inner_def
 fst_l_def snd_l_def prio_l_def option_l_def triv_l_def
@@ -1256,6 +486,14 @@ fst_l_def snd_l_def prio_l_def option_l_def triv_l_def
 option_ok_S prod_ok_S prio_ok_S triv_ok_S oalist_ok_S
  LNew_def
 split: md_triv.splits) 
+
+  apply(force simp add: calc_lift'_def schem_lift_defs merge_l_def mem_lift1_def
+mem_sem_lifting_inner_def
+fst_l_def snd_l_def prio_l_def option_l_def triv_l_def
+option_ok_S prod_ok_S prio_ok_S triv_ok_S oalist_ok_S
+ LNew_def
+split: md_triv.splits) 
+
 
     done
 
@@ -1446,7 +684,7 @@ option_ok_S prod_ok_S prio_ok_S triv_ok_S oalist_ok_S
 split: md_triv.splits) 
     done
 
-  obtain Inv :: "(_ :: {Bogus,Okay,Mergeableb,Pordc_all}) Mem_Simple.state1 \<Rightarrow> bool" where Inv_def :
+  obtain Inv :: "(_ :: {Bogus,Okay,Mergeableb,Pordc_all, Pordps}) Mem_Simple.state1 \<Rightarrow> bool" where Inv_def :
   "Inv = (\<lambda> st . st \<in> ok_S \<and> (case st of
                      (reg_flag, reg_c, reg_a, reg_b,  m, xz) \<Rightarrow>
                       (case m of
@@ -1675,6 +913,18 @@ split: md_triv.splits option.splits)
 and P' = "\<lambda> _ . True"
 in Calc_Final)
 *)
+(* TODO: looks like we actually do need a fact about the rest of the state
+remaining unchanged. (this is in cases like arith, for instance, we need
+to show a sort of "frame" where everything not in calc is unchanged *)
+
+(*
+    apply(rule_tac P = ?B2
+and P' = "\<lambda> st . case st of (reg_a, reg_b, reg_c) \<Rightarrow>
+          reg_a = i1 \<and>
+          (\<exists> (idx :: int) . i2 \<ge> idx \<and> idx > 0 \<and> reg_b = i1 * (i2 - idx))"
+in Calc_Final)
+*)
+
     apply(rule_tac P = ?B2
 and P' = "\<lambda> st . case st of (reg_a, reg_b, reg_c) \<Rightarrow>
           reg_a = i1 \<and>
@@ -1728,13 +978,21 @@ split: md_triv.splits)
 
     apply(clarify)
     apply(simp (no_asm_simp))
+(* begin experiment *)
 
+
+(* end experiment *)
   apply(simp add: Inv_def cond_lift'_def calc_lift'_def schem_lift_defs merge_l_def mem_lift1_def
 mem_sem_lifting_inner_def
 fst_l_def snd_l_def prio_l_def option_l_def triv_l_def
 option_ok_S prod_ok_S prio_ok_S triv_ok_S oalist_ok_S
  LNew_def split: md_triv.splits
 ) 
+
+    apply(clarify)
+
+    apply(auto split: md_triv.splits)
+(* idxb vs idx *)
 
     done
 
